more stuff

src/ra.v
@@ -8,28 +8,23 @@ From iris.proofmode Require Import ltac_tactics.
 From iris.proofmode Require Import tactics.
 From iris.proofmode Require Import coq_tactics.
 
-
-
 From stdpp Require Import gmap.
 From stdpp Require Import mapset.
 From stdpp Require Import sets.
 From stdpp Require Import list.
 Require Import Burrow.gmap_utils.
 Require Import Burrow.tactics.
-Require Import Burrow.resource_proofs.
 Require Import Burrow.locations.
 Require Import Burrow.rollup.
+Require Import Burrow.tpcms.
+Require Import Burrow.resource_proofs.
 Require Import coq_tricks.Deex.
 
-Global Instance state_pcore
-        M `{!EqDecision M} `{!TPCM M}
-        RI `{!EqDecision RI} `{!Countable RI} `{!RefinementIndex M RI}
-      : PCore (State M RI) := λ state , Some state_unit.
+Global Instance state_pcore (𝜇 : BurrowCtx)
+      : PCore (BurrowState 𝜇) := λ state , Some state_unit.
 
-Definition burrow_ra_mixin
-        M `{!EqDecision M} `{!TPCM M}
-        RI `{!EqDecision RI, !Countable RI, !RefinementIndex M RI}
-    : RAMixin (State M RI).
+Definition burrow_ra_mixin (𝜇: BurrowCtx)
+    : RAMixin (BurrowState 𝜇).
 Proof. split.
   - typeclasses eauto.
   - unfold pcore. unfold state_pcore. intros. exists cx. split; trivial.
@@ -37,7 +32,7 @@ Proof. split.
   - typeclasses eauto.
   - typeclasses eauto.
   - unfold pcore. unfold state_pcore. intros.
-      replace cx with state_unit by crush.
+      inversion H.
       setoid_rewrite state_comm.
       apply op_state_unit.
   - unfold pcore. unfold state_pcore. intros. rewrite H. unfold "≡", option_equiv.
@@ -52,74 +47,77 @@ Proof. split.
 Defined.
 
 Global Instance State_equivalence
-    M `{!EqDecision M} `{!TPCM M}
-    RI `{!EqDecision RI} `{!Countable RI} `{!RefinementIndex M RI}
-  : Equivalence (≡@{State M RI}).
+    (𝜇: BurrowCtx)
+  : Equivalence (≡@{BurrowState 𝜇}).
 Proof. split; typeclasses eauto. Defined.
 
 Canonical Structure burrowO
-    M `{!EqDecision M} `{!TPCM M}
-    RI `{!EqDecision RI} `{!Countable RI} `{!RefinementIndex M RI}
-  := discreteO (State M RI).
+    (𝜇: BurrowCtx)
+  := discreteO (BurrowState 𝜇).
 
 Canonical Structure burrowR
-    M `{!EqDecision M} `{!TPCM M}
-    RI `{!EqDecision RI} `{!Countable RI} `{!RefinementIndex M RI}
-    := discreteR (State M RI) (burrow_ra_mixin M RI).
+    (𝜇: BurrowCtx)
+    := discreteR (BurrowState 𝜇) (burrow_ra_mixin 𝜇).
     
-    
-Context M `{!EqDecision M} `{!TPCM M}.
-Context RI `{!EqDecision RI} `{!Countable RI} `{!RefinementIndex M RI}.
+Context {𝜇: BurrowCtx}.
     
 Class gen_burrowGpreS (Σ : gFunctors) := {
-  gen_burrowGpreS_inG :> inG Σ (burrowR M RI);
+  gen_burrowGpreS_inG :> inG Σ (burrowR 𝜇);
 }.
 
 Class gen_burrowGS (Σ : gFunctors) := GenBurrowGS {
   gen_burrow_inG :> gen_burrowGpreS Σ;
   gen_burrow_name : gname;
 }.
-Print gen_burrow_name.
 Global Arguments GenBurrowGS Σ {_} _ : assert.
 Global Arguments gen_burrow_name {Σ} _ : assert.
 
 Definition gen_burrowΣ : gFunctors := #[
-  GFunctor (burrowR M RI)
+  GFunctor (burrowR 𝜇)
 ].
 
 Global Instance subG_gen_burrowGpreS {Σ} :
   subG (gen_burrowΣ) Σ → gen_burrowGpreS Σ.
 Proof. solve_inG. Qed.
 
-Definition L (𝛾: Loc RI) (m: M) : iProp Σ
-    := own (gen_burrow_name hG) (live 𝛾 m).
+Context `{hG : !gen_burrowGS Σ}.
+
+Definition L
+    {M} `{!EqDecision M} `{!TPCM M} `{!HasTPCM 𝜇 M}
+    (𝛾: BurrowLoc 𝜇) (m: M) : iProp Σ
+    := own (gen_burrow_name hG) (live' 𝛾 m).
     
-Definition R (𝜅: Lifetime) (𝛾: Loc RI) (m: M) : iProp Σ
-    := own (gen_burrow_name hG) (reserved 𝜅 𝛾 m) ∧ ⌜ 𝜅 ≠ empty_lifetime ⌝.
+Definition R
+    {M} `{!EqDecision M} `{!TPCM M} `{!HasTPCM 𝜇 M}
+    (𝜅: Lifetime) (𝛾: BurrowLoc 𝜇) (m: M) : iProp Σ
+    := own (gen_burrow_name hG) (reserved' 𝜅 𝛾 m) ∧ ⌜ 𝜅 ≠ empty_lifetime ⌝.
     
-Definition B (𝜅: Lifetime) (𝛾: Loc RI) (m: M) : iProp Σ
+Definition B
+    {M} `{!EqDecision M} `{!TPCM M} `{!HasTPCM 𝜇 M}
+    (𝜅: Lifetime) (𝛾: BurrowLoc 𝜇) (m: M) : iProp Σ
     := ∃ rstate ,
         own (gen_burrow_name hG) rstate ∧
-        ⌜ is_borrow 𝜅 𝛾 m rstate /\ state_no_live rstate ⌝.
+        ⌜ is_borrow' 𝜅 𝛾 m rstate /\ state_no_live rstate ⌝.
 
 Definition A (𝜅: Lifetime) : iProp Σ
-    := own (gen_burrow_name hG) (active 𝜅).
+    := own (gen_burrow_name hG) (active 𝜅 : BurrowState 𝜇).
 
-Global Instance burrow_cmra_discrete : CmraDiscrete (burrowR M RI).
+Global Instance burrow_cmra_discrete : CmraDiscrete (burrowR 𝜇).
 Proof. apply discrete_cmra_discrete. Qed.
 
-Global Instance burrow_cmra_total : CmraTotal (burrowR M RI).
+Global Instance burrow_cmra_total : CmraTotal (burrowR 𝜇).
 Proof. unfold CmraTotal. intros. unfold pcore, cmra_pcore, burrowR, state_pcore.
   unfold is_Some. exists state_unit. trivial.
 Qed.
 
 Lemma BorrowExpire
-  (𝜅: Lifetime) (𝛾: Loc RI) (m: M)
+    {M} `{!EqDecision M} `{!TPCM M} `{!HasTPCM 𝜇 M}
+    (𝜅: Lifetime) (𝛾: BurrowLoc 𝜇) (m: M)
   : A 𝜅 ∗ R 𝜅 𝛾 m ==∗ L 𝛾 m.
 Proof. unfold A, R, L.
   iIntros "[H1 [H2 %H3]]". 
   iCombine "H1" "H2" as "H".
-  iMod (own_update (gen_burrow_name hG) (active 𝜅 ⋅ reserved 𝜅 𝛾 m) (live 𝛾 m) with "H") as "$".
+  iMod (own_update (gen_burrow_name hG) ((active 𝜅: BurrowState 𝜇) ⋅ reserved' 𝜅 𝛾 m) (live' 𝛾 m) with "H") as "$".
   - have h := cmra_discrete_update.
     rewrite cmra_discrete_update.
     intro. apply borrow_expire. trivial.
